feat: simplify over applied terms

tests/lean/run/sym_simp_1.lean
@@ -59,3 +59,55 @@ example (h : HEq a = f) : HEq (α := Nat) (0 + a) = f := by
   sym_simp [Nat.zero_add]
   trace_state
   exact h
+
+/--
+trace: a b : Nat
+f : Nat → Nat
+h : f a = b
+⊢ id f a = b
+-/
+#guard_msgs in
+example (f : Nat → Nat) (h : f a = b) : id f (0 + a) = b := by
+  sym_simp [Nat.zero_add]
+  trace_state
+  exact h
+
+def f (_ : α) {β : Type} (b : β) : β := b
+
+/--
+trace: a : Nat
+g : Nat → Nat
+⊢ f 0 g a = g a
+-/
+#guard_msgs in
+example (g : Nat → Nat) : f (0 + 0) g (0 + a) = g a := by
+  sym_simp [Nat.zero_add]
+  trace_state
+  rfl
+
+def f' (_ : α) (b : β) := b
+
+/--
+trace: a : Nat
+g : Nat → Nat
+⊢ f' 0 g a = g a
+-/
+#guard_msgs in
+example (g : Nat → Nat) : f' (0 + 0) g (0 + a) = g a := by
+  sym_simp [Nat.zero_add]
+  trace_state
+  rfl
+
+/--
+trace: a b : Nat
+as : Array (Nat → Nat)
+i : Nat
+x✝ : i < as.size
+h : as[i] a = b
+⊢ as[i] a = b
+-/
+#guard_msgs in
+example (as : Array (Nat → Nat)) (i : Nat) (_ : i < as.size) (h : as[i] a = b) : as[0 + i] (0 + a) = b := by
+  sym_simp [Nat.zero_add]
+  trace_state
+  exact h
